version with Program Fixpoint instead of refine
seems to be about 10x slower, though; will probably revert to refine

coq/two/LambdaTwo.v
@@ -1,26 +1,9 @@
-Require Import Recdef.
-Require Export LambdaTwoSyntax.
-Require Export IndistinguishabilityTwo.
+Require Import Coq.Program.Wf.
 Require Import LibTactics.
-Require Import Wf_nat.
+Require Export LambdaTwoSyntax IndistinguishabilityTwo.
 
 Definition pair_lt (a b : nat * nat) : Prop :=
   fst a + snd a < fst b + snd b.
-
-Lemma pair_lt_wf' :
-  forall s a, fst a + snd a <= s -> Acc pair_lt a.
-Proof.
-  induction s; intros a H1.
-  - destruct a as [a1 a2]; destruct a1; destruct a2; auto.
-    apply Acc_intro. intros y H2. inversion H2.
-  - inversion H1 as [H2 | n H2 Heq]; auto.
-    apply Acc_intro. intros y H3. inversion H3; auto.
-Defined.
-
-Theorem pair_lt_wf : well_founded pair_lt.
-Proof.
-  unfold well_founded; intro; eapply pair_lt_wf'; eauto.
-Defined.
 
 Definition bottomp : forall l : two, {l = Bottom2} + {l = Top2} :=
   fun (l : two) =>
@@ -34,54 +17,76 @@ Example bottomp_example :
   (if bottomp Top2 then 1 else 2) = 2.
 Proof. split; reflexivity. Qed.
 
-Definition eval_kl : nat * nat -> two -> (value -> value -> Prop) ->
-                     two -> env -> term -> atom -> Prop.
-  refine
-    (Fix pair_lt_wf (fun _ => two -> (value -> value -> Prop) ->
-                              two -> env -> term -> atom -> Prop)
-         (fun (kl : nat * nat)
-              (eval_kl : forall kl' : nat * nat,
-                           pair_lt kl' kl ->
-                           two -> (value -> value -> Prop) ->
-                           two -> env -> term -> atom -> Prop) =>
-            fun (L : two) (P : value -> value -> Prop)
-                (pc : two) (e : env) (t : term) (a : atom) =>
-              match t with
-                | TBool b =>
-                  a = Atom (VBool b) pc
-                | TNat n =>
-                  a = Atom (VNat n) pc
-                | TVar n =>
-                  exists v l,
-                    atIndex e n = Some (Atom v l) /\
-                    a = Atom v (l ⊔ pc)
-                | TAbs t' =>
-                  a = Atom (VClos e t') pc
-                | TApp t1 t2 =>
-                  if Compare_dec.zerop (fst kl) then False
-                  else let eval := eval_kl (fst kl - 1, snd kl) _ in
-                       exists e1' t1' l1 a2 a3,
-                         eval L P pc e t1 (Atom (VClos e1' t1') l1) /\
-                         eval L P pc e t2 a2 /\
-                         eval L P l1 (a2 :: e1') t1' a3 /\
-                         a = a3
-                | TDecl t1 t2 =>
-                  if Compare_dec.zerop (fst kl) then False
-                  else let eval := eval_kl (fst kl - 1, snd kl) _ in
-                       exists e1' t1' l1 a2 v3 l3,
-                         eval L P pc e t1 (Atom (VClos e1' t1') l1) /\
-                         eval L P pc e t2 a2 /\
-                         eval L P l1 (a2 :: e1') t1' (Atom v3 l3) /\
-                         if bottomp l3 then a = Atom v3 Bottom2
-                         else let eval := eval_kl (snd kl, fst kl - 1) _ in
-                              (forall a2' e2' v3',
-                                 env_LPequiv L P (a2 :: e1') (a2' :: e2') ->
-                                 eval L P l1 (a2' :: e2') t1' (Atom v3' Top2) ->
-                                 value_LPequiv L P v3 v3') /\
-                              a = Atom v3 Bottom2
-              end));
-  unfold pair_lt; simpl; omega.
+Program Fixpoint eval_kl (kl : nat * nat) (L : two) (P : value -> value -> Prop)
+        (pc : two) (e : env) (t : term) (a : atom) {wf pair_lt kl} : Prop :=
+  match t with
+    | TBool b =>
+      a = Atom (VBool b) pc
+    | TNat n =>
+      a = Atom (VNat n) pc
+    | TVar n =>
+      exists v l,
+        atIndex e n = Some (Atom v l) /\
+        a = Atom v (l ⊔ pc)
+    | TAbs t' =>
+      a = Atom (VClos e t') pc
+    | TApp t1 t2 =>
+      if Compare_dec.zerop (fst kl) then False
+      else let eval := eval_kl (fst kl - 1, snd kl) in
+           exists e1' t1' l1 a2 a3,
+             eval L P pc e t1 (Atom (VClos e1' t1') l1) _ /\
+             eval L P pc e t2 a2 _ /\
+             eval L P l1 (a2 :: e1') t1' a3 _ /\
+             a = a3
+    | TDecl t1 t2 =>
+      if Compare_dec.zerop (fst kl) then False
+      else let eval := eval_kl (fst kl - 1, snd kl) in
+           exists e1' t1' l1 a2 v3 l3,
+             eval L P pc e t1 (Atom (VClos e1' t1') l1) _ /\
+             eval L P pc e t2 a2 _ /\
+             eval L P l1 (a2 :: e1') t1' (Atom v3 l3) _ /\
+             if bottomp l3 then a = Atom v3 Bottom2
+             else let eval := eval_kl (snd kl, fst kl - 1) in
+                  (forall a2' e2' v3',
+                     env_LPequiv L P (a2 :: e1') (a2' :: e2') ->
+                     eval L P l1 (a2' :: e2') t1' (Atom v3' Top2) _ ->
+                     value_LPequiv L P v3 v3') /\
+                  a = Atom v3 Bottom2
+  end.
+
+Obligation 1. unfold pair_lt. simpl in *. omega. Qed.
+Obligation 2. unfold pair_lt. simpl in *. omega. Qed.
+Obligation 3. unfold pair_lt. simpl in *. omega. Qed.
+Obligation 4. unfold pair_lt. simpl in *. omega. Qed.
+Obligation 5. unfold pair_lt. simpl in *. omega. Qed.
+Obligation 6. unfold pair_lt. simpl in *. omega. Qed.
+Obligation 7. unfold pair_lt. simpl in *. omega. Qed.
+
+Definition eval_kl_type : Type :=
+  {_ : nat * nat & {_ : two & {_ : value -> value -> Prop &
+  {_ : two & {_ : env & {_ : term & atom}}}}}}.
+
+Lemma eval_kl_wf' :
+  forall s a,
+    fst (projT1 a) + snd (projT1 a) <= s ->
+    Acc (fun x y : eval_kl_type => pair_lt (projT1 x) (projT1 y)) a.
+Proof.
+  induction s; intros a H1.
+  - destruct a as [a1 a2]; destruct a1; destruct a2; inversion H1.
+    apply Acc_intro. intros y H2. inversion H2.
+    + rewrite H0 in H3. inversion H3.
+    + rewrite H0 in H. inversion H.
+  - inversion H1 as [H2 | n H2 Heq]; auto.
+    apply Acc_intro. intros y H3. inversion H3; apply IHs; omega.
 Defined.
+
+Theorem eval_kl_wf :
+  well_founded (fun x y : eval_kl_type => pair_lt (projT1 x) (projT1 y)).
+Proof.
+  unfold well_founded; intro; eapply eval_kl_wf'; eauto.
+Defined.
+
+Obligation 8. unfold well_founded. intro. eapply eval_kl_wf'. eauto. Defined.
 
 Definition eval (L : two) (P : value -> value -> Prop)
            (pc : two) (e : env) (t : term) (a : atom) : Prop :=
@@ -91,7 +96,7 @@ Lemma eval_kl_bool :
   forall k l L P pc e b,
     eval_kl (k, l) L P pc e (TBool b) (Atom (VBool b) pc).
 Proof.
-  introv. destruct k; destruct l; repeat red; auto.
+  introv. destruct k. destruct l. reflexivity. reflexivity. reflexivity.
 Qed.
 
 Lemma eval_kl_bool_inv :
@@ -101,14 +106,14 @@ Lemma eval_kl_bool_inv :
 Proof.
   introv Heval.
   destruct a as [v1 l1]; destruct v1 as [b1 | n1 | e1 t1];
-  destruct k; destruct l; inversion Heval; auto.
+  destruct k; destruct l; inversion Heval; reflexivity.
 Qed.
 
 Lemma eval_kl_nat :
   forall k l L P pc e n,
     eval_kl (k, l) L P pc e (TNat n) (Atom (VNat n) pc).
 Proof.
-  introv. destruct k; destruct l; repeat red; auto.
+  introv. destruct k. destruct l. reflexivity. reflexivity. reflexivity.
 Qed.
 
 Lemma eval_kl_nat_inv :
@@ -118,7 +123,7 @@ Lemma eval_kl_nat_inv :
 Proof.
   introv Heval.
   destruct a as [v1 l1]; destruct v1 as [b1 | n1 | e1 t1];
-  destruct k; destruct l; inversion Heval; auto.
+  destruct k; destruct l; inversion Heval; reflexivity.
 Qed.
 
 Lemma eval_kl_var :
@@ -126,7 +131,8 @@ Lemma eval_kl_var :
     atIndex e n = Some (Atom v' l') ->
     eval_kl (k, l) L P pc e (TVar n) (Atom v' (l' ⊔ pc)).
 Proof.
-  introv He. destruct k; destruct l; repeat red; exists v' l'; auto.
+  introv He. destruct k. destruct l.
+  exists v' l'. auto. exists v' l'. auto. exists v' l'. auto.
 Qed.
 
 Lemma eval_kl_var_inv :
@@ -145,7 +151,7 @@ Lemma eval_kl_abs :
   forall k l L P pc e t',
     eval_kl (k, l) L P pc e (TAbs t') (Atom (VClos e t') pc).
 Proof.
-  introv. destruct k; destruct l; repeat red; auto.
+  introv. destruct k. destruct l. reflexivity. reflexivity. reflexivity.
 Qed.
   
 Lemma eval_kl_abs_inv :
@@ -155,7 +161,7 @@ Lemma eval_kl_abs_inv :
 Proof.
   introv Heval.
   destruct a as [v1 l1]; destruct v1 as [b1 | n1 | e1 t1];
-  destruct k; destruct l; inversion Heval; auto.
+  destruct k; destruct l; inversion Heval; reflexivity.
 Qed.
 
 Lemma eval_kl_app :
